First attempt at reverting to old-style time delayed used in operational semantics.

src/SymbolicPrimitive.thy
@@ -32,16 +32,12 @@ datatype cnt_expr =
 
 subsection\<open> Symbolic Primitives for Runs \<close>
 
-text\<open>
-  Tag values are used to refer to the time on a clock at a given instant index.
-\<close>
-datatype tag_val =
-  TSchematic \<open>clock * instant_index\<close> (\<open>\<tau>\<^sub>v\<^sub>a\<^sub>r\<close>)
-
 datatype '\<tau> constr =
 \<comment> \<open>@{term \<open>c \<Down> n @ \<tau>\<close>} constrains clock @{term \<open>c\<close>} to have time @{term \<open>\<tau>\<close>}
     at instant @{term \<open>n\<close>} of the run.\<close>
   Timestamp     \<open>clock\<close>   \<open>instant_index\<close> \<open>'\<tau> tag_const\<close>         (\<open>_ \<Down> _ @ _\<close>)
+(* TODO: comments *)
+| Timestamp2    \<open>clock\<close>   \<open>instant_index\<close> \<open>'\<tau> tag_expr\<close>          (\<open>_ \<Down> _ @@ _\<close>)
 \<comment> \<open>@{term \<open>m @ n \<oplus> \<delta>t \<Rightarrow> s\<close>} constrains clock @{term \<open>s\<close>} to tick at the
     first instant at which the time on @{term \<open>m\<close>} has increased by @{term \<open>\<delta>t\<close>}
     from the value it had at instant @{term \<open>n\<close>} of the run.\<close>
@@ -108,6 +104,7 @@ where
 | \<open>\<lbrakk> K \<not>\<Up> < n \<rbrakk>\<^sub>p\<^sub>r\<^sub>i\<^sub>m   = {\<rho>. \<forall>i < n. \<not> ticks ((Rep_run \<rho>) i K)}\<close>
 | \<open>\<lbrakk> K \<not>\<Up> \<ge> n \<rbrakk>\<^sub>p\<^sub>r\<^sub>i\<^sub>m   = {\<rho>. \<forall>i \<ge> n. \<not> ticks ((Rep_run \<rho>) i K) }\<close>
 | \<open>\<lbrakk> K \<Down> n @ \<tau> \<rbrakk>\<^sub>p\<^sub>r\<^sub>i\<^sub>m = {\<rho>. time ((Rep_run \<rho>) n K) = \<tau> }\<close>
+| \<open>\<lbrakk> K \<Down> n @@ \<lparr>\<tau>\<^sub>v\<^sub>a\<^sub>r(K', n') \<oplus> \<delta>\<tau>\<rparr> \<rbrakk>\<^sub>p\<^sub>r\<^sub>i\<^sub>m = {\<rho>. time ((Rep_run \<rho>) n K) = time ((Rep_run \<rho>) n' K') + \<delta>\<tau> }\<close>
 | \<open>\<lbrakk> \<lfloor>\<tau>\<^sub>v\<^sub>a\<^sub>r(K\<^sub>1, n\<^sub>1), \<tau>\<^sub>v\<^sub>a\<^sub>r(K\<^sub>2, n\<^sub>2)\<rfloor> \<in> R \<rbrakk>\<^sub>p\<^sub>r\<^sub>i\<^sub>m =
     { \<rho>. R (time ((Rep_run \<rho>) n\<^sub>1 K\<^sub>1), time ((Rep_run \<rho>) n\<^sub>2 K\<^sub>2)) }\<close>
 | \<open>\<lbrakk> \<lceil>e\<^sub>1, e\<^sub>2\<rceil> \<in> R \<rbrakk>\<^sub>p\<^sub>r\<^sub>i\<^sub>m = { \<rho>. R (\<lbrakk> \<rho> \<turnstile> e\<^sub>1 \<rbrakk>\<^sub>c\<^sub>n\<^sub>t\<^sub>e\<^sub>x\<^sub>p\<^sub>r, \<lbrakk> \<rho> \<turnstile> e\<^sub>2 \<rbrakk>\<^sub>c\<^sub>n\<^sub>t\<^sub>e\<^sub>x\<^sub>p\<^sub>r) }\<close>
