src/Operational.thy
@@ -87,6 +87,7 @@ where
     forbidding a tick on the slave clock.\<close>
   \<open>(\<Gamma>, n \<turnstile> ((K\<^sub>1 implies not K\<^sub>2) # \<Psi>) \<triangleright> \<Phi>)
      \<hookrightarrow>\<^sub>e  (((K\<^sub>1 \<Up> n) # (K\<^sub>2 \<not>\<Up> n) # \<Gamma>), n \<turnstile> \<Psi> \<triangleright> ((K\<^sub>1 implies not K\<^sub>2) # \<Phi>))\<close>
+(* Targets stutter-invariance *)
 | timedelayed_e1:
 \<comment> \<open>A timed delayed implication can be handled by forbidding a tick on 
     the master clock.\<close>
@@ -98,6 +99,13 @@ where
   \<open>(\<Gamma>, n \<turnstile> ((K\<^sub>1 time-delayed by \<delta>\<tau> on K\<^sub>2 implies K\<^sub>3) # \<Psi>) \<triangleright> \<Phi>)
      \<hookrightarrow>\<^sub>e  (((K\<^sub>1 \<Up> n) # (K\<^sub>2 @ n \<oplus> \<delta>\<tau> \<Rightarrow> K\<^sub>3) # \<Gamma>), n
             \<turnstile> \<Psi> \<triangleright> ((K\<^sub>1 time-delayed by \<delta>\<tau> on K\<^sub>2 implies K\<^sub>3) # \<Phi>))\<close>
+(* Targets operational use *)
+| timedelayed2_e1:
+  \<open>(\<Gamma>, n \<turnstile> ((K\<^sub>1 time-delayed2 by \<delta>\<tau> on K\<^sub>2 implies K\<^sub>3) # \<Psi>) \<triangleright> \<Phi>)
+     \<hookrightarrow>\<^sub>e  (((K\<^sub>1 \<not>\<Up> n) # \<Gamma>), n \<turnstile> \<Psi> \<triangleright> ((K\<^sub>1 time-delayed2 by \<delta>\<tau> on K\<^sub>2 implies K\<^sub>3) # \<Phi>))\<close>
+| timedelayed2_e2:
+  \<open>(\<Gamma>, n \<turnstile> ((K\<^sub>1 time-delayed2 by \<delta>\<tau> on K\<^sub>2 implies K\<^sub>3) # \<Psi>) \<triangleright> \<Phi>)
+     \<hookrightarrow>\<^sub>e  (((K\<^sub>1 \<Up> n) # \<Gamma>), n \<turnstile> ((K\<^sub>3 sporadic-add \<lparr>\<tau>\<^sub>v\<^sub>a\<^sub>r(K\<^sub>2, n) \<oplus> \<delta>\<tau>\<rparr> on K\<^sub>2) # \<Psi>) \<triangleright> ((K\<^sub>1 time-delayed2 by \<delta>\<tau> on K\<^sub>2 implies K\<^sub>3) # \<Phi>))\<close>
 | weakly_precedes_e:
 \<comment> \<open>A weak precedence relation has to hold at every instant.\<close>
   \<open>(\<Gamma>, n \<turnstile> ((K\<^sub>1 weakly precedes K\<^sub>2) # \<Psi>) \<triangleright> \<Phi>)
